proved simple regex = accept in the other derection, forgot that the privious time

poregexML.sml
@@ -1,0 +1,36 @@
+structure poregexML :> poregexML =
+struct
+  nonfix accept parts split Rep Seq Alt Sym Eps * / div mod + - ^ @ <> >
+         < >= <= := o before;
+
+  open listML
+
+  datatype 'a Reg
+       = Eps
+       | Sym of 'a
+       | Alt of 'a Reg * 'a Reg
+       | Seq of 'a Reg * 'a Reg
+       | Rep of 'a Reg
+  fun split [] = [([],[])]
+    | split (c::cs) =
+        ([],c::cs)::
+        MAP (fn x => (c::pairML.FST x,pairML.SND x)) (split cs)
+
+  fun parts [] = [[]]
+    | parts (c::cs) =
+        (if cs = [] then
+           [[[c]]]
+         else FLAT (MAP (fn x => [[c]::x,(c::HD x)::TL x]) (parts cs)))
+
+  fun accept Eps u = (u = [])
+    | accept (Sym(c)) u = (u = [c])
+    | accept (Alt(p,q)) u = accept p u orelse accept q u
+    | accept (Seq(p,q)) u =
+        EXISTS (fn x =>
+          accept p (pairML.FST x) andalso accept q (pairML.SND x))
+          (split u)
+    | accept (Rep(r)) u =
+        EXISTS (fn partition =>
+          EVERY (fn part => accept r part) partition) (parts u)
+
+end
